skeletons/skeletons.v
@@ -1,0 +1,262 @@
+(* Add LoadPath "C:\Users\Ziga\Documents\Ziga_podatki\repositories\eeff-formalization\syntax". *)
+(* Add LoadPath "C:\Users\Ziga\Documents\Ziga_podatki\repositories\eeff-formalization\type_system". *)
+(* Add LoadPath "C:\Users\Ziga\Documents\Ziga_podatki\repositories\eeff-formalization\substitution". *)
+Add LoadPath "E:\Ziga_Podatki\faks\eeff-formalization\syntax".
+Add LoadPath "E:\Ziga_Podatki\faks\eeff-formalization\type_system".
+Add LoadPath "E:\Ziga_Podatki\faks\eeff-formalization\substitution".
+Require Export declarational.
+
+(* ==================== Syntax ==================== *)
+
+Inductive sk_vtype : Type :=
+| SkTyUnit : sk_vtype
+| SkTyInt : sk_vtype
+| SkTyØ : sk_vtype
+| SkTyΣ : sk_vtype -> sk_vtype -> sk_vtype
+| SkTyΠ : sk_vtype -> sk_vtype -> sk_vtype
+| SkTyList : sk_vtype -> sk_vtype
+| SkTyFun : sk_vtype -> sk_ctype -> sk_vtype
+| SkTyHandler : sk_ctype -> sk_ctype -> sk_vtype
+
+with sk_ctype : Type :=
+| SkCTy : sk_vtype -> sk_ctype
+.
+
+Inductive sk_val : Type :=
+| SkVar : nat -> sk_val
+| SkUnit : sk_val
+| SkInt : Z.t -> sk_val
+| SkInl : sk_val -> sk_val
+| SkInr : sk_val -> sk_val
+| SkPair : sk_val -> sk_val -> sk_val
+| SkListNil : sk_val
+| SkListCons : sk_val -> sk_val -> sk_val
+| SkFun : sk_comp -> sk_val
+| SkHandler : sk_comp -> sk_hcases -> sk_val
+
+with sk_comp : Type :=
+| SkRet : sk_val -> sk_comp
+| SkAbsurd : sk_val -> sk_comp
+| SkΠMatch : sk_val -> sk_comp -> sk_comp
+| SkΣMatch : sk_val -> sk_comp -> sk_comp -> sk_comp
+| SkListMatch : sk_val -> sk_comp -> sk_comp -> sk_comp
+| SkApp : sk_val -> sk_val -> sk_comp
+| SkOp : op_id -> sk_vtype -> sk_vtype -> sk_val -> sk_comp -> sk_comp
+| SkLetRec : sk_comp -> sk_comp -> sk_comp
+| SkDoBind : sk_comp -> sk_comp -> sk_comp
+| SkHandle : sk_val -> sk_comp -> sk_comp
+
+with sk_hcases : Type :=
+| SkCasesØ : sk_hcases
+| SkCasesU : sk_hcases -> op_id -> sk_vtype -> sk_vtype -> sk_comp -> sk_hcases
+.
+
+Inductive sk_ctx : Type :=
+| SkCtxØ : sk_ctx
+| SkCtxU : sk_ctx -> sk_vtype -> sk_ctx
+.
+
+Fixpoint get_sk_vtype Γ i :=
+  match Γ, i with
+  | SkCtxØ , _=> None
+  | SkCtxU Γ' A, 0 => Some A
+  | SkCtxU Γ' A, S i' =>  get_sk_vtype Γ' i'
+  end.
+
+(* ==================== Type Judgements ==================== *)
+
+Inductive has_sk_vtype : sk_ctx -> sk_val -> sk_vtype -> Prop :=
+| SkTypeUnit Γ : 
+    has_sk_vtype Γ SkUnit SkTyUnit 
+| SkTypeInt Γ n : 
+    has_sk_vtype Γ (SkInt n) SkTyInt
+| SkTypeVar Γ n A :
+    get_sk_vtype Γ n = Some A ->
+    has_sk_vtype Γ (SkVar n) A
+| SkTypePair Γ v1 v2 A B :
+    has_sk_vtype Γ v1 A ->
+    has_sk_vtype Γ v2 B ->
+    has_sk_vtype Γ (SkPair v1 v2) (SkTyΠ A B)
+| SkTypeInl Γ v A B :
+    has_sk_vtype Γ v A ->
+    has_sk_vtype Γ (SkInl v) (SkTyΣ A B)
+| SkTypeInr Γ v A B :
+    has_sk_vtype Γ v B ->
+    has_sk_vtype Γ (SkInr v) (SkTyΣ A B)
+| SkTypeListNil Γ A :
+    has_sk_vtype Γ SkListNil (SkTyList A)
+| SkTypeListCons Γ v vs A :
+    has_sk_vtype Γ v A ->
+    has_sk_vtype Γ vs (SkTyList A) ->
+    has_sk_vtype Γ (SkListCons v vs) (SkTyList A)
+| SkTypeFun Γ c A C :
+    has_sk_ctype (SkCtxU Γ A) c C ->
+    has_sk_vtype Γ (SkFun c) (SkTyFun A C)
+| SkTypeHandler Γ cr h A D :
+    has_sk_ctype (SkCtxU Γ A) cr D ->
+    has_sk_htype Γ h D -> 
+    has_sk_vtype Γ (SkHandler cr h) (SkTyHandler (SkCTy A) D)
+
+with has_sk_ctype : sk_ctx -> sk_comp -> sk_ctype -> Prop :=
+| SkTypeRet Γ v A : 
+    has_sk_vtype Γ v A ->
+    has_sk_ctype Γ (SkRet v) (SkCTy A)
+| SkTypeAbsurd Γ v C :
+    has_sk_vtype Γ v SkTyØ -> 
+    has_sk_ctype Γ (SkAbsurd v) C
+| SkTypeΠMatch Γ v A B c C :
+    has_sk_vtype Γ v (SkTyΠ A B) ->
+    has_sk_ctype (SkCtxU (SkCtxU Γ A) B) c C ->
+    has_sk_ctype Γ (SkΠMatch v c) C
+| SkTypeΣMatch Γ v A B c1 c2 C :
+    has_sk_vtype Γ v (SkTyΣ A B) ->
+    has_sk_ctype (SkCtxU Γ A) c1 C ->
+    has_sk_ctype (SkCtxU Γ B) c2 C ->
+    has_sk_ctype Γ (SkΣMatch v c1 c2) C
+| SkTypeListMatch Γ v A c1 c2 C :
+    has_sk_vtype Γ v (SkTyList A) ->
+    has_sk_ctype Γ c1 C ->
+    has_sk_ctype (SkCtxU (SkCtxU Γ A) (SkTyList A)) c2 C ->
+    has_sk_ctype Γ (SkListMatch v c1 c2) C
+| SkTypeDoBind Γ c1 c2 A B :
+    has_sk_ctype Γ c1 (SkCTy A) ->
+    has_sk_ctype (SkCtxU Γ A) c2 (SkCTy B) ->
+    has_sk_ctype Γ (SkDoBind c1 c2) (SkCTy B)
+| SkTypeApp Γ v1 v2 A C :
+    has_sk_vtype Γ v1 (SkTyFun A C) ->
+    has_sk_vtype Γ v2 A ->
+    has_sk_ctype Γ (SkApp v1 v2) C
+| SkTypeHandle Γ v c C D :
+    has_sk_vtype Γ v (SkTyHandler C D) ->
+    has_sk_ctype Γ c C ->
+    has_sk_ctype Γ (SkHandle v c) D
+| SkTypeLetRec Γ A C c1 c2 D:
+    has_sk_ctype (SkCtxU (SkCtxU Γ A) (SkTyFun A C)) c1 C ->
+    has_sk_ctype (SkCtxU Γ (SkTyFun A C)) c2 D ->
+    has_sk_ctype Γ (SkLetRec c1 c2) D
+| SkTypeOp Γ op v c Aop Bop A :
+    has_sk_vtype Γ v Aop ->
+    has_sk_ctype (SkCtxU Γ Bop) c (SkCTy A) ->
+    has_sk_ctype Γ (SkOp op Aop Bop v c) (SkCTy A)
+
+with has_sk_htype : sk_ctx -> sk_hcases -> sk_ctype -> Prop :=
+| SkTypeCasesØ Γ D : has_sk_htype Γ SkCasesØ D
+| SkTypeCasesU Γ h op cop Aop Bop D :
+    has_sk_htype Γ h D ->
+    has_sk_ctype (SkCtxU (SkCtxU Γ Aop) (SkTyFun Bop D)) cop D ->
+    has_sk_htype Γ (SkCasesU h op Aop Bop cop) D
+.
+
+
+(* ==================== Necromancy ==================== *)
+
+Fixpoint skeletize_vtype A :=
+  match A with
+  | TyUnit => SkTyUnit
+  | TyInt => SkTyInt
+  | TyØ => SkTyØ
+  | TyΣ A B => SkTyΣ (skeletize_vtype A) (skeletize_vtype B)
+  | TyΠ A B => SkTyΠ (skeletize_vtype A) (skeletize_vtype B)
+  | TyList A => SkTyList (skeletize_vtype A)
+  | TyFun A C => SkTyFun (skeletize_vtype A) (skeletize_ctype C)
+  | TyHandler C D => SkTyHandler (skeletize_ctype C) (skeletize_ctype D)
+  end
+with skeletize_ctype C :=
+  match C with
+  | CTy A Σ E => SkCTy (skeletize_vtype A)
+  end
+.
+
+Fixpoint skeletize_ctx Γ :=
+  match Γ with
+  | CtxØ => SkCtxØ
+  | CtxU Γ A => SkCtxU (skeletize_ctx Γ) (skeletize_vtype A)
+  end.
+
+(* The variable 'p' is the proof term. We do that to avoid constructing proof
+   terms by hand. This might complicate things later on, since it breaks
+   proof dependency by introducing new proofs. *)
+
+Inductive v_ann : forall Γ v A, has_vtype Γ v A -> sk_val -> Prop :=
+| AnnVar Γ n A p:
+    get_vtype Γ n = Some A ->
+    v_ann Γ (Var n) A p (SkVar n)
+| AnnUnit Γ p: 
+    v_ann Γ Unit TyUnit p SkUnit
+| AnnInt Γ n p: 
+    v_ann Γ (Int n) TyInt p (SkInt n)
+| AnnPair Γ v1 v2 A B v1' v2' p1 p2 p:
+    v_ann Γ v1 A p1 v1' -> v_ann Γ v2 B p2 v2' ->
+    v_ann Γ (Pair v1 v2) (TyΠ A B) p (SkPair v1' v2')
+| AnnInl Γ v A B v' pl p:
+    v_ann Γ v A pl v' ->
+    v_ann Γ (Inl v) (TyΣ A B) p (SkInl v')
+| AnnInr Γ v A B v' pr p:
+    v_ann Γ v B pr v' ->
+    v_ann Γ (Inr v) (TyΣ A B) p (SkInr v')
+| AnnListNil Γ A p:
+    v_ann Γ ListNil (TyList A) p (SkListNil)
+| AnnListCons Γ v1 v2 A v1' v2' p1 p2 p:
+    v_ann Γ v1 A p1 v1' -> v_ann Γ v2 (TyList A) p2 v2' ->
+    v_ann Γ (ListCons v1 v2) (TyList A) p (SkListCons v1' v2')
+| AnnFun Γ c A C c' pc p:
+    c_ann (CtxU Γ A) c C pc c' ->
+    v_ann Γ (Fun c) (TyFun A C) p (SkFun c')
+| AnnHandler Γ c c' h h' A Σ E D pc ph p:
+    c_ann (CtxU Γ A) c D pc c' -> h_ann Γ h Σ D ph h' ->
+    v_ann Γ (Handler c h) (TyHandler (CTy A Σ E) D) p (SkHandler c' h')
+| AnnVSubtype Γ v v' A A' p p':
+    v_ann Γ v A p' v' ->
+    vsubtype A A' ->
+    v_ann Γ v A' p v'
+
+with c_ann : forall Γ c C, has_ctype Γ c C -> sk_comp -> Prop :=
+| AnnRet Γ v v' A pv p :
+    v_ann Γ v A pv v' ->
+    c_ann Γ (Ret v) (CTy A SigØ EqsØ) p (SkRet v')
+| AnnAbsurd Γ v v' C pv p :
+    v_ann Γ v TyØ pv v' ->
+    c_ann Γ (Absurd v) C p (SkAbsurd v')
+| AnnΠMatch Γ v v' A B c c' C pv pc p:
+    v_ann Γ v (TyΠ A B) pv v' -> c_ann (CtxU (CtxU Γ A) B) c C pc c'->
+    c_ann Γ (ΠMatch v c) C p (SkΠMatch v' c')
+| AnnΣMatch Γ v v' A B c1 c1' c2 c2' C p pv pc1 pc2:
+    v_ann Γ v (TyΣ A B) pv v' ->
+    c_ann (CtxU Γ A) c1 C pc1 c1' -> c_ann (CtxU Γ B) c2 C pc2 c2' ->
+    c_ann Γ (ΣMatch v c1 c2) C p (SkΣMatch v' c1' c2')
+| AnnListMatch Γ v v' A c1 c1' c2 c2' C p pv pc1 pc2:
+    v_ann Γ v (TyList A) pv v' ->
+    c_ann Γ c1 C pc1 c1' -> c_ann (CtxU (CtxU Γ A) (TyList A)) c2 C pc2 c2' ->
+    c_ann Γ (ListMatch v c1 c2) C p (SkListMatch v' c1' c2')
+| AnnDoBind Γ c1 c1' c2 c2' A B Σ E p pc1 pc2:
+    c_ann Γ c1 (CTy A Σ E) pc1 c1' -> c_ann (CtxU Γ A) c2 (CTy B Σ E) pc2 c2' ->
+    c_ann Γ (DoBind c1 c2) (CTy B Σ E) p (SkDoBind c1' c2')
+| AnnApp Γ v1 v1' v2 v2' A C pv1 pv2 p:
+    v_ann Γ v1 (TyFun A C) pv1 v1' -> v_ann Γ v2 A pv2 v2' ->
+    c_ann Γ (App v1 v2) C p (SkApp v1' v2')
+| AnnHandle Γ v v' c c' C D pv pc p:
+    v_ann Γ v (TyHandler C D) pv v' -> c_ann Γ c C pc c' ->
+    c_ann Γ (Handle v c) D p (SkHandle v' c')
+| AnnLetRec Γ c1 c1' c2 c2' A C D pc1 pc2 p :
+    c_ann (CtxU (CtxU Γ A) (TyFun A C)) c1 C pc1 c1' ->
+    c_ann (CtxU Γ (TyFun A C)) c2 D pc2 c2' -> 
+    c_ann Γ (LetRec c1 c2) D p (SkLetRec c1' c2')
+| AnnOp Γ op v v' c c' A Σ E Aop Bop pv pc p :
+    get_op_type Σ op = Some (Aop, Bop) ->
+    v_ann Γ v Aop pv v' -> c_ann (CtxU Γ Bop) c (CTy A Σ E) pc c' ->
+    c_ann Γ (Op op v c) (CTy A Σ E) p 
+      (SkOp op (skeletize_vtype Aop) (skeletize_vtype Bop) v' c')
+| AnnCSubtype Γ c c' C C' p p':
+    c_ann Γ c C p' c' ->
+    csubtype C C' ->
+    c_ann Γ c C' p c'
+
+with h_ann : forall Γ h Σ D, has_htype Γ h Σ D -> sk_hcases -> Prop := 
+| AnnCasesØ Γ Σ D p:
+    h_ann Γ CasesØ Σ D p SkCasesØ
+| AnnCasesU Γ Σ D h h' c c' A B op ph pc p:
+    h_ann Γ h Σ D ph h' ->
+    c_ann (CtxU (CtxU Γ A) (TyFun B D)) c D pc c' ->
+    h_ann Γ (CasesU h op A B c) (SigU Σ op A B) D p 
+      (SkCasesU h' op (skeletize_vtype A) (skeletize_vtype B) c')
+.
